dataplane/AntichainOrder.thy
@@ -218,18 +218,6 @@ lemma frontier_add_zmset:
   using frontier_below_eq_frontier_plus_pos
   by (metis add_zmset_add_single dual_order.refl dual_order.trans zcount_single zero_less_one_class.zero_le_one)
 
-
-(*
-\<forall>t. 0 < zcount (c_pts (pt_tr sg) (Loc 1 (Trg 1))) t + zcount (zmset (map snd (filter (\<lambda>(l', t, d). Loc 1 (Trg 1) = l') (lo_pt sg)))) t + zcount (zmset (map snd (produ os1))) t +
-            zcount (zmset (map snd (filter (\<lambda>(l', t, d). Loc 1 (Trg 1) = l') (map (\<lambda>(p, t, m). (Loc 1 (Trg 1), t, - m)) (consu os2))))) t +
-            (if n 1 = t then zcount {#}\<^sub>z t + 1 else zcount {#}\<^sub>z t) \<longrightarrow>
-        t \<le> n 1 \<Longrightarrow>
-    frontier
-     (c_pts (pt_tr sg) (Loc 1 (Trg 1)) + zmset (map snd (filter (\<lambda>(l', t, d). Loc 1 (Trg 1) = l') (lo_pt sg))) +
-      (zmset (map snd (produ os1)) + (zmset (map snd (filter (\<lambda>(l', t, d). Loc 1 (Trg 1) = l') (map (\<lambda>(p, t, m). (Loc 1 (Trg 1), t, - m)) (consu os2)))) + {#n 1#}\<^sub>z)))
-    \<le> frontier (zmset_of {#n 1. x \<in># mset batch'#})
-*)
-
 lemma frontier_le_add_singleton:
   "(\<forall>t'. zcount A t' > 0 \<longrightarrow> t' \<le> t) \<Longrightarrow>
    (zcount A t \<ge> 0) \<Longrightarrow>
@@ -286,24 +274,6 @@ lemma frontier_le_zmset_of[simp]:
   apply (induct xs)
   using frontier_le_add apply fastforce+
   done
-
-(*
-frontier
-     (add_zmset (n 1)
-       (c_pts (pt_tr sg) (Loc 1 (Trg 1)) + zmset (map snd (filter (\<lambda>(l', t, d). Loc 1 (Trg 1) = l') (lo_pt sg))) + zmset (map snd (produ os1)) +
-        zmset (map snd (filter (\<lambda>(l', t, d). Loc 1 (Trg 1) = l') (map (\<lambda>(p, t, m). (Loc 1 (Trg 1), t, - m)) (consu os2))))))
-    \<le> frontier {#n 1#}\<^sub>z \<Longrightarrow>
-    frontier
-     (add_zmset (n 1)
-       (c_pts (pt_tr sg) (Loc 1 (Trg 1)) + zmset (map snd (filter (\<lambda>(l', t, d). Loc 1 (Trg 1) = l') (lo_pt sg))) + zmset (map snd (produ os1)) +
-        zmset (map snd (filter (\<lambda>(l', t, d). Loc 1 (Trg 1) = l') (map (\<lambda>(p, t, m). (Loc 1 (Trg 1), t, - m)) (consu os2))))))
-    \<le> frontier
-        (add_zmset (n 1)
-          (c_pts (pt_tr sg) (Loc 1 (Trg 1)) + zmset (map snd (filter (\<lambda>(l', t, d). Loc 1 (Trg 1) = l') (lo_pt sg))) +
-           (zmset (map snd (produ os1)) + (zmset (map snd (filter (\<lambda>(l', t, d). Loc 1 (Trg 1) = l') (map (\<lambda>(p, t, m). (Loc 1 (Trg 1), t, - m)) (consu os2)))) + zmset_of {#n 1. x \<in># mset batch'#}))))
-
-*)
-
 
 lemma frontie_add_zmset_add:
   "frontier (add_zmset t A) \<le> frontier {#t#}\<^sub>z \<Longrightarrow>
